implemented R C T sets

ASC_Suite.thy
@@ -2,11 +2,16 @@ theory ASC_Suite
 imports ASC_LB
 begin
 
-(* maximum length contained common prefix *)
+(* maximum length contained prefix *)
 fun mcp :: "'a list \<Rightarrow> 'a list set \<Rightarrow> 'a list \<Rightarrow> bool" where
+  "mcp z W p = (prefix p z \<and> p \<in> W \<and> 
+                 (\<forall> p' . (prefix p' z \<and> p' \<in> W) \<longrightarrow> length p' \<le> length p))"
+
+(* def. for contained common prefix :
   "mcp z W p = (p \<in> {p . prefix p z \<and> (\<exists> w \<in> W . prefix p w)}
                 \<and> (\<forall> p' \<in> {p . prefix p z \<and> (\<exists> w \<in> W . prefix p w)} .
                   length p' \<le> length p))"
+*)
 
 lemma mcp_ex :
   assumes "[] \<in> W"
@@ -14,11 +19,10 @@ lemma mcp_ex :
 obtains p
 where "mcp z W p"  
 proof -
-  let ?P = "{p . prefix p z \<and> (\<exists> w \<in> W . prefix p w)}"
+  let ?P = "{p . prefix p z \<and> p \<in> W}"
   let ?maxP = "arg_max length (\<lambda> p . p \<in> ?P)"
 
-  have "?P \<subseteq> {p . prefix p z} \<union> {p . \<exists> w \<in> W . prefix p w}" by blast
-  moreover have "finite {p . prefix p z}" 
+  have "finite {p . prefix p z}" 
   proof -
     have "{p . prefix p z} \<subseteq> image (\<lambda> i . take i z) (set [0 ..< Suc (length z)])"
     proof 
@@ -31,9 +35,7 @@ proof -
     qed
     then show ?thesis using finite_surj by blast 
   qed
-  moreover have "finite {p . \<exists> w \<in> W . prefix p w}"
-    by (metis (no_types) List.finite_set assms(2) finite_Collect_bex set_prefixes_eq) 
-  ultimately have "finite ?P" by simp 
+  then have "finite ?P" by simp 
 
   have "?P \<noteq> {}"
     using Nil_prefix assms(1) by blast 
@@ -55,6 +57,102 @@ proof -
   then show ?thesis using that by auto
 qed
 
+
+lemma mcp_unique :
+  assumes "mcp z W p" 
+  and     "mcp z W p'"
+shows "p = p'"
+proof -
+  have "length p' \<le> length p" using assms(1) assms(2) by auto 
+  moreover have "length p \<le> length p'" using assms(1) assms(2) by auto
+  ultimately have "length p' = length p" by simp
+
+  moreover have "prefix p z" using assms(1) by auto
+  moreover have "prefix p' z" using assms(2) by auto
+  ultimately show ?thesis by (metis append_eq_conv_conj prefixE)
+qed
+
+fun mcp' :: "'a list \<Rightarrow> 'a list set \<Rightarrow> 'a list" where
+  "mcp' z W = (THE p . mcp z W p)"
+
+lemma mcp'_intro : 
+  assumes "mcp z W p"
+shows "mcp' z W = p"
+using assms mcp_unique by (metis mcp'.elims theI_unique) 
+
+
+fun N :: "('in \<times> 'out) list \<Rightarrow> ('in, 'out, 'state) FSM \<Rightarrow> 'in list set \<Rightarrow> ('in \<times> 'out) list set set" where
+  "N io M V = { V'' \<in> Perm V M . (map fst (mcp' io V'')) = (mcp' (map fst io) V) }"
+(*
+  "N io M V = { V'' \<in> Perm V M . \<exists> vs \<in> V'' . (mcp' (map fst io) V) = map fst vs 
+                                              \<and> prefix vs io }"
+*)
+(*
+  "N io M V = { V'' \<in> Perm V M . \<exists> v . prefix v (map fst io) \<and> 
+                            (\<forall> w . prefix w (map fst io) \<longrightarrow> (length w > length v \<longrightarrow> w \<notin> V))
+                            \<and> (\<exists> v' . length v' = length v \<and> (v || v') \<in> V'' \<and> prefix (v || v') io)}"
+*)
+
+(* TODO - show that construction is nonempty
+lemma N_nonempty :
+  assumes "[] \<in> V"
+  shows "N io M V \<noteq> {}"
+*)
+
+(* Corollary 7.1.2 *)
+lemma x :
+  assumes "map fst vs = mcp' (map fst (vs@xs)) V"
+  and     "V'' \<in> N (vs@xs) M1 V"
+  and     "is_det_state_cover M2 V"
+  and     "well_formed M2"
+  and     "finite V"
+shows "vs \<in> V'' \<and> vs = mcp' (vs@xs) V''" 
+proof 
+  have "map fst (mcp' (vs@xs) V'') = mcp' (map fst (vs@xs)) V" using assms(2) by auto
+  then have "map fst (mcp' (vs@xs) V'') = map fst vs" using assms(1) by presburger
+  then have "length (mcp' (vs@xs) V'') = length vs" by (metis length_map) 
+
+  have "[] \<in> V''" using perm_empty[OF assms(3)] N.simps assms(2) by blast 
+  moreover have "finite V''" using perm_elem_finite[OF assms(3,4)] N.simps assms(2) by blast
+  ultimately obtain p where "mcp (vs@xs) V'' p" using mcp_ex by auto 
+  then have "mcp' (vs@xs) V'' = p" using mcp'_intro by simp
+  
+
+  then have "prefix (mcp' (vs@xs) V'') (vs@xs)" unfolding mcp'.simps mcp.simps
+    using \<open>mcp (vs @ xs) V'' p\<close> mcp.elims(2) by blast 
+  then show "vs = mcp' (vs@xs) V''"
+    by (metis \<open>length (mcp' (vs @ xs) V'') = length vs\<close> append_eq_append_conv prefix_def) 
+
+  show "vs \<in> V''"
+    using \<open>mcp (vs @ xs) V'' p\<close> \<open>mcp' (vs @ xs) V'' = p\<close> \<open>vs = mcp' (vs @ xs) V''\<close> by auto 
+qed
+
+
+
+
+
+fun TS :: "('in, 'out, 'state1) FSM \<Rightarrow> ('in, 'out, 'state2) FSM \<Rightarrow> 'in list set \<Rightarrow> 'state1 set \<Rightarrow> ('in, 'out) ATC set \<Rightarrow> 'in list set \<Rightarrow> nat \<Rightarrow> 'in list set" 
+and C  :: "('in, 'out, 'state1) FSM \<Rightarrow> ('in, 'out, 'state2) FSM \<Rightarrow> 'in list set \<Rightarrow> 'state1 set \<Rightarrow> ('in, 'out) ATC set \<Rightarrow> 'in list set \<Rightarrow> nat \<Rightarrow> 'in list set"   
+and R  :: "('in, 'out, 'state1) FSM \<Rightarrow> ('in, 'out, 'state2) FSM \<Rightarrow> 'in list set \<Rightarrow> 'state1 set \<Rightarrow> ('in, 'out) ATC set \<Rightarrow> 'in list set \<Rightarrow> nat \<Rightarrow> 'in list set"   
+where
+  "R M2 M1 T S \<Omega> V 0 = {}" |
+  "TS M2 M1 T S \<Omega> V 0 = V" |
+  "TS M2 M1 T S \<Omega> V (Suc 0) = V" |
+  "C M2 M1 T S \<Omega> V 0 = V" |
+  "C M2 M1 T S \<Omega> V (Suc 0) = V" |
+  "R M2 M1 T S \<Omega> V (Suc n) = 
+    {xs' \<in> C M2 M1 T S \<Omega> V (Suc n) .
+      (\<exists> vs xs . (vs@xs) \<in> language_state_in M1 (initial M1) {xs'}
+        \<and> (\<exists> S1 . S1 \<subseteq> S
+          \<and> (\<exists> V'' \<in> N (vs@xs) M1 V . 
+            vs = mcp' (vs@xs) V''
+            \<and> (\<forall> s1 \<in> S1 . \<forall> s2 \<in> S1 .
+              s1 \<noteq> s2 \<longrightarrow> 
+                (\<forall> io1 \<in> RP M2 s1 vs xs V'' .
+                   \<forall> io2 \<in> RP M2 s2 vs xs V'' .
+                     B M1 io1 \<Omega> \<noteq> B M1 io2 \<Omega> )))))}" |
+  "C M2 M1 T S \<Omega> V (Suc n) = { xs@[x] | xs x . xs \<in> ((C M2 M1 T S \<Omega> V n) - (R M2 M1 T S \<Omega> V n)) \<and> x : inputs M2 } - (TS M2 M1 T S \<Omega> V n)" |
+  "TS M2 M1 T S \<Omega> V (Suc n) = (TS M2 M1 T S \<Omega> V n) \<union> (C M2 M1 T S \<Omega> V (Suc n))" 
     
     
 
